Fix POPLmark typing

thys/POPLmark/SystemFSub.thy
@@ -205,7 +205,9 @@ inductive ty :: "'a::var \<Gamma>\<^sub>\<tau> \<Rightarrow> 'a typ \<Rightarrow
 | SA_Trans_TVar: "\<lbrakk> x<:U \<in> \<Gamma> ; \<Gamma> \<turnstile> U <: T \<rbrakk> \<Longrightarrow> \<Gamma> \<turnstile> TyVar x <: T"
 | SA_Arrow: "\<lbrakk> \<Gamma> \<turnstile> T\<^sub>1 <: S\<^sub>1 ; \<Gamma> \<turnstile> S\<^sub>2 <: T\<^sub>2 \<rbrakk> \<Longrightarrow> \<Gamma> \<turnstile> S\<^sub>1 \<rightarrow> S\<^sub>2 <: T\<^sub>1 \<rightarrow> T\<^sub>2"
 | SA_All: "\<lbrakk> \<Gamma> \<turnstile> T\<^sub>1 <: S\<^sub>1 ; \<Gamma>\<^bold>, x<:T\<^sub>1 \<turnstile> S\<^sub>2 <: T\<^sub>2 \<rbrakk> \<Longrightarrow> \<Gamma> \<turnstile> \<forall>x<:S\<^sub>1. S\<^sub>2 <: \<forall>x<:T\<^sub>1 .T\<^sub>2"
-| SA_Rec: "\<lbrakk> \<turnstile> \<Gamma> ok; labels X \<subseteq> labels Y; \<And>x T. (x, T) \<in>\<in> Y \<Longrightarrow> \<exists>S. (x, S) \<in>\<in> X \<and> \<Gamma> \<turnstile> S <: T\<rbrakk> \<Longrightarrow> \<Gamma> \<turnstile> Rec X <: Rec Y"
+| SA_Rec: "\<lbrakk> \<turnstile> \<Gamma> ok; labels Y \<subseteq> labels X;
+    \<And>x T. (x, T) \<in>\<in> X \<Longrightarrow> T closed_in \<Gamma> ;
+    \<And>x T. (x, T) \<in>\<in> Y \<Longrightarrow> \<exists>S. (x, S) \<in>\<in> X \<and> \<Gamma> \<turnstile> S <: T \<rbrakk> \<Longrightarrow> \<Gamma> \<turnstile> Rec X <: Rec Y"
 
 inductive_cases
   SA_TopE[elim!]: "\<Gamma> \<turnstile> Top <: T"
@@ -239,29 +241,21 @@ using assms proof (induction \<Gamma> S T rule: ty.induct)
     case 2 then show ?case using SA_Trans_TVar by simp
   }
 next
-  case (SA_Rec \<Gamma> X Y)
+  case (SA_Rec \<Gamma> Y X)
   {
     case 1
     then show ?case unfolding typ.set
     proof safe
       fix x T
-      assume "T \<in> values X" "x \<in> FVars_typ T"
-      from \<open>T \<in> values X\<close> obtain l where "(l, T) \<in>\<in> X"
+      assume a: "T \<in> values X" "x \<in> FVars_typ T"
+      from \<open>T \<in> values X\<close> obtain l where 1: "(l, T) \<in>\<in> X"
         by (meson values_lfin)
-      with SA_Rec(2) obtain U where "(l, U) \<in>\<in> Y"
-        including lfset.lifting
-        by transfer auto
-      with SA_Rec(3) obtain T' where "(l, T') \<in>\<in> X" "T' closed_in \<Gamma>"
-        by blast
-      moreover from \<open>Pair l T \<in>\<in> X\<close> \<open>(l, T') \<in>\<in> X\<close> have "T = T'"
-        by (simp add: lfin_label_inject)
-      ultimately show "x \<in> dom \<Gamma>" using \<open>x \<in> FVars_typ T\<close>
-        by auto
+      then show "x \<in> dom \<Gamma>" using SA_Rec(3) a by fast
     qed
   next
     case 2
     then show ?case unfolding typ.set
-      by (auto dest!: values_lfin SA_Rec(3))
+      by (auto dest!: values_lfin SA_Rec(4))
   }
 qed auto
 
